\begin{frame}[fragile]{Meta LMM}
			
	\begin{equation*}
		\begin{aligned}	
			y_{ijk} \sim LogNormal(\mu_{ijk}, \sigma_{e_k}^2)\\
			\mu_{ijk} = \alpha_k + \beta_k \cdot x_{[0,1]} + u_i + w_j\\
			\alpha_k = \alpha_{\mu} + \alpha_{\tau} \cdot \alpha_{\eta_k}\\
			\beta_k = \beta_{\mu} + \beta_{\tau} \cdot \beta_{\eta_k}\\
			\text{constraint: }\sigma_{e_k}^2>0\\
		\end{aligned}	
	\end{equation*}		
	\begin{small}	
		\begin{itemize}
			\item $x=0$ for simple NPs; $x=1$ for conjoined NPs.
		\end{itemize}
	\end{small}
	
\end{frame}

\begin{frame}[fragile]{Meta LMM (unequal variance)}
	\begin{equation*}
		\begin{aligned}
			y_{ijk} \sim
			\begin{dcases*} 
				LogNormal(\mu_{ijk}, \sigma_{e_k}^2), &  if NP$_{i}$ = simple\\
				LogNormal(\mu_{ijk} + \beta_k, \sigma_{e'_k}^2) & else if NP$_{i}$ = conjoined\\
			\end{dcases*}\\
			\mu_{ijk} = \alpha_k + u_i + w_j\\
			\alpha_k = \alpha_{\mu} + \alpha_{\tau} \cdot \alpha_{\eta_k}\\
			\beta_k = \beta_{\mu} + \beta_{\tau} \cdot \beta_{\eta_k}\\
			\text{constraint: }\sigma_{e_k}^2>0\\
			\sigma_{e'_k}^2 > \sigma_{e_k}^2
		\end{aligned}
	\end{equation*}

\end{frame}


\begin{frame}[fragile]{Meta mixture model (alternative hypothesis)}

	\begin{equation*}
		\begin{aligned}
		y_{ijk} \sim \theta_{{NP}_k} \cdot LogNormal(\mu_{ijk} + \delta_k, \sigma_{e'_k}^2) + \\
			(1 - \theta_{{NP}_k}) \cdot LogNormal(\mu_{ijk}, \sigma_{e_k}^2) \\
			\mu_{ijk} = \alpha_k + u_i + w_j\\
			\alpha_k = \alpha_{\mu} + \alpha_{\tau} \cdot \alpha_{\eta_k}\\
			\theta_{{NP}_k} = Logit^{-1}(\phi_{{NP}_k})\\
			\theta_{\mu_{NP}} = Logit^{-1}(\phi_{_{\mu_{NP}}})\\		
			\phi_{{NP}_k} \sim Normal(\phi_{\mu_{NP}}, \phi_{\tau}^2)\\
			\delta_k \sim Normal(\delta_{\mu}, \delta_{\tau}^2)\\
			\text{constraint: }\delta_k, \sigma_{e_k}^2, \phi_{\tau}, \delta_{\tau}>0\\
			\sigma_{e'_k}^2 > \sigma_{e_k}^2 
		\end{aligned}
	\end{equation*}
	
\end{frame}


